dijkstra/dijkstra1.v
@@ -72,15 +72,15 @@ Definition ___stringlit_3 : ident := 104%positive.
 Definition ___stringlit_4 : ident := 105%positive.
 Definition ___stringlit_5 : ident := 111%positive.
 Definition ___stringlit_6 : ident := 112%positive.
-Definition _argc : ident := 120%positive.
-Definition _argv : ident := 121%positive.
+Definition _argc : ident := 121%positive.
+Definition _argv : ident := 122%positive.
 Definition _arr : ident := 66%positive.
 Definition _capacity : ident := 5%positive.
 Definition _cells : ident := 77%positive.
-Definition _cost : ident := 118%positive.
+Definition _cost : ident := 119%positive.
 Definition _curr : ident := 107%positive.
 Definition _data : ident := 3%positive.
-Definition _dijkstra : ident := 119%positive.
+Definition _dijkstra : ident := 120%positive.
 Definition _dist : ident := 110%positive.
 Definition _exch : ident := 70%positive.
 Definition _fa : ident := 76%positive.
@@ -100,7 +100,7 @@ Definition _key : ident := 1%positive.
 Definition _key1 : ident := 68%positive.
 Definition _key2 : ident := 69%positive.
 Definition _key_table : ident := 8%positive.
-Definition _keys : ident := 117%positive.
+Definition _keys : ident := 118%positive.
 Definition _less : ident := 73%positive.
 Definition _lookup : ident := 67%positive.
 Definition _main : ident := 92%positive.
@@ -115,6 +115,7 @@ Definition _pq_insert : ident := 86%positive.
 Definition _pq_insert_nc : ident := 78%positive.
 Definition _pq_make : ident := 90%positive.
 Definition _pq_remove_min : ident := 87%positive.
+Definition _pq_remove_min_nc : ident := 85%positive.
 Definition _pq_size : ident := 72%positive.
 Definition _prev : ident := 108%positive.
 Definition _printPath : ident := 109%positive.
@@ -123,7 +124,6 @@ Definition _printf : ident := 95%positive.
 Definition _priority : ident := 2%positive.
 Definition _rand : ident := 93%positive.
 Definition _random : ident := 99%positive.
-Definition _remove_min_nc : ident := 85%positive.
 Definition _setup : ident := 100%positive.
 Definition _sink : ident := 75%positive.
 Definition _size : ident := 88%positive.
@@ -134,20 +134,20 @@ Definition _structPQ : ident := 9%positive.
 Definition _swim : ident := 74%positive.
 Definition _table : ident := 80%positive.
 Definition _target : ident := 81%positive.
+Definition _the_item : ident := 117%positive.
 Definition _time : ident := 96%positive.
 Definition _u : ident := 114%positive.
-Definition _t'1 : ident := 122%positive.
-Definition _t'10 : ident := 131%positive.
-Definition _t'11 : ident := 132%positive.
-Definition _t'12 : ident := 133%positive.
-Definition _t'2 : ident := 123%positive.
-Definition _t'3 : ident := 124%positive.
-Definition _t'4 : ident := 125%positive.
-Definition _t'5 : ident := 126%positive.
-Definition _t'6 : ident := 127%positive.
-Definition _t'7 : ident := 128%positive.
-Definition _t'8 : ident := 129%positive.
-Definition _t'9 : ident := 130%positive.
+Definition _t'1 : ident := 123%positive.
+Definition _t'10 : ident := 132%positive.
+Definition _t'11 : ident := 133%positive.
+Definition _t'2 : ident := 124%positive.
+Definition _t'3 : ident := 125%positive.
+Definition _t'4 : ident := 126%positive.
+Definition _t'5 : ident := 127%positive.
+Definition _t'6 : ident := 128%positive.
+Definition _t'7 : ident := 129%positive.
+Definition _t'8 : ident := 130%positive.
+Definition _t'9 : ident := 131%positive.
 
 Definition v___stringlit_4 := {|
   gvar_info := (tarray tschar 22);
@@ -501,16 +501,15 @@ Definition f_dijkstra := {|
   fn_params := ((_graph, (tptr (tptr tint))) :: (_src, tint) ::
                 (_dist, (tptr tint)) :: (_prev, (tptr tint)) ::
                 (_size, tint) :: (_inf, tint) :: nil);
-  fn_vars := nil;
+  fn_vars := ((_the_item, (Tstruct _structItem noattr)) :: nil);
   fn_temps := ((_i_ptr, (tptr tint)) :: (_keys, (tptr tint)) ::
                (_pq, (tptr (Tstruct _structPQ noattr))) :: (_i, tint) ::
-               (_j, tint) :: (_u, tint) :: (_cost, tint) :: (_t'6, tint) ::
-               (_t'5, (tptr (Tstruct _structItem noattr))) ::
+               (_j, tint) :: (_u, tint) :: (_cost, tint) :: (_t'5, tint) ::
                (_t'4, tuint) :: (_t'3, tuint) ::
                (_t'2, (tptr (Tstruct _structPQ noattr))) ::
-               (_t'1, (tptr tvoid)) :: (_t'12, tint) :: (_t'11, tint) ::
-               (_t'10, tint) :: (_t'9, tint) :: (_t'8, tint) ::
-               (_t'7, tint) :: nil);
+               (_t'1, (tptr tvoid)) :: (_t'11, tint) :: (_t'10, tint) ::
+               (_t'9, tint) :: (_t'8, tint) :: (_t'7, tint) ::
+               (_t'6, tint) :: nil);
   fn_body :=
 (Ssequence
   (Ssequence
@@ -575,7 +574,7 @@ Definition f_dijkstra := {|
                 (tptr tint)) tint) (Etempvar _src tint))
           (Ssequence
             (Ssequence
-              (Sset _t'12
+              (Sset _t'11
                 (Ederef
                   (Ebinop Oadd (Etempvar _keys (tptr tint))
                     (Etempvar _src tint) (tptr tint)) tint))
@@ -586,7 +585,7 @@ Definition f_dijkstra := {|
                                             (Tcons tint (Tcons tint Tnil)))
                                           tvoid cc_default))
                 ((Etempvar _pq (tptr (Tstruct _structPQ noattr))) ::
-                 (Etempvar _t'12 tint) :: (Econst_int (Int.repr 0) tint) ::
+                 (Etempvar _t'11 tint) :: (Econst_int (Int.repr 0) tint) ::
                  nil)))
             (Ssequence
               (Sloop
@@ -604,113 +603,116 @@ Definition f_dijkstra := {|
                       Sskip
                       Sbreak))
                   (Ssequence
+                    (Scall None
+                      (Evar _pq_remove_min_nc (Tfunction
+                                                (Tcons
+                                                  (tptr (Tstruct _structPQ noattr))
+                                                  (Tcons
+                                                    (tptr (Tstruct _structItem noattr))
+                                                    Tnil)) tvoid cc_default))
+                      ((Etempvar _pq (tptr (Tstruct _structPQ noattr))) ::
+                       (Eaddrof (Evar _the_item (Tstruct _structItem noattr))
+                         (tptr (Tstruct _structItem noattr))) :: nil))
                     (Ssequence
-                      (Scall (Some _t'5)
-                        (Evar _pq_remove_min (Tfunction
-                                               (Tcons
-                                                 (tptr (Tstruct _structPQ noattr))
-                                                 Tnil)
-                                               (tptr (Tstruct _structItem noattr))
-                                               cc_default))
-                        ((Etempvar _pq (tptr (Tstruct _structPQ noattr))) ::
-                         nil))
                       (Sset _u
-                        (Efield
-                          (Ederef
-                            (Etempvar _t'5 (tptr (Tstruct _structItem noattr)))
-                            (Tstruct _structItem noattr)) _data tint)))
-                    (Ssequence
-                      (Sset _i (Econst_int (Int.repr 0) tint))
-                      (Sloop
-                        (Ssequence
-                          (Sifthenelse (Ebinop Olt (Etempvar _i tint)
-                                         (Etempvar _size tint) tint)
-                            Sskip
-                            Sbreak)
+                        (Efield (Evar _the_item (Tstruct _structItem noattr))
+                          _data tint))
+                      (Ssequence
+                        (Sset _i (Econst_int (Int.repr 0) tint))
+                        (Sloop
                           (Ssequence
+                            (Sifthenelse (Ebinop Olt (Etempvar _i tint)
+                                           (Etempvar _size tint) tint)
+                              Sskip
+                              Sbreak)
                             (Ssequence
-                              (Scall (Some _t'6)
-                                (Evar _getCell (Tfunction
-                                                 (Tcons (tptr (tptr tint))
-                                                   (Tcons tint
-                                                     (Tcons tint Tnil))) tint
-                                                 cc_default))
-                                ((Etempvar _graph (tptr (tptr tint))) ::
-                                 (Etempvar _u tint) :: (Etempvar _i tint) ::
-                                 nil))
-                              (Sset _cost (Etempvar _t'6 tint)))
-                            (Sifthenelse (Ebinop Olt (Etempvar _cost tint)
-                                           (Etempvar _inf tint) tint)
                               (Ssequence
-                                (Sset _t'7
-                                  (Ederef
-                                    (Ebinop Oadd (Etempvar _dist (tptr tint))
-                                      (Etempvar _i tint) (tptr tint)) tint))
+                                (Scall (Some _t'5)
+                                  (Evar _getCell (Tfunction
+                                                   (Tcons (tptr (tptr tint))
+                                                     (Tcons tint
+                                                       (Tcons tint Tnil)))
+                                                   tint cc_default))
+                                  ((Etempvar _graph (tptr (tptr tint))) ::
+                                   (Etempvar _u tint) ::
+                                   (Etempvar _i tint) :: nil))
+                                (Sset _cost (Etempvar _t'5 tint)))
+                              (Sifthenelse (Ebinop Olt (Etempvar _cost tint)
+                                             (Etempvar _inf tint) tint)
                                 (Ssequence
-                                  (Sset _t'8
+                                  (Sset _t'6
                                     (Ederef
                                       (Ebinop Oadd
                                         (Etempvar _dist (tptr tint))
-                                        (Etempvar _u tint) (tptr tint)) tint))
-                                  (Sifthenelse (Ebinop Ogt
-                                                 (Etempvar _t'7 tint)
-                                                 (Ebinop Oadd
-                                                   (Etempvar _t'8 tint)
-                                                   (Etempvar _cost tint)
-                                                   tint) tint)
-                                    (Ssequence
+                                        (Etempvar _i tint) (tptr tint)) tint))
+                                  (Ssequence
+                                    (Sset _t'7
+                                      (Ederef
+                                        (Ebinop Oadd
+                                          (Etempvar _dist (tptr tint))
+                                          (Etempvar _u tint) (tptr tint))
+                                        tint))
+                                    (Sifthenelse (Ebinop Ogt
+                                                   (Etempvar _t'6 tint)
+                                                   (Ebinop Oadd
+                                                     (Etempvar _t'7 tint)
+                                                     (Etempvar _cost tint)
+                                                     tint) tint)
                                       (Ssequence
-                                        (Sset _t'11
-                                          (Ederef
-                                            (Ebinop Oadd
-                                              (Etempvar _dist (tptr tint))
-                                              (Etempvar _u tint) (tptr tint))
-                                            tint))
-                                        (Sassign
-                                          (Ederef
-                                            (Ebinop Oadd
-                                              (Etempvar _dist (tptr tint))
-                                              (Etempvar _i tint) (tptr tint))
-                                            tint)
-                                          (Ebinop Oadd (Etempvar _t'11 tint)
-                                            (Etempvar _cost tint) tint)))
-                                      (Ssequence
-                                        (Sassign
-                                          (Ederef
-                                            (Ebinop Oadd
-                                              (Etempvar _prev (tptr tint))
-                                              (Etempvar _i tint) (tptr tint))
-                                            tint) (Etempvar _u tint))
                                         (Ssequence
-                                          (Sset _t'9
+                                          (Sset _t'10
                                             (Ederef
                                               (Ebinop Oadd
-                                                (Etempvar _keys (tptr tint))
-                                                (Etempvar _i tint)
+                                                (Etempvar _dist (tptr tint))
+                                                (Etempvar _u tint)
                                                 (tptr tint)) tint))
+                                          (Sassign
+                                            (Ederef
+                                              (Ebinop Oadd
+                                                (Etempvar _dist (tptr tint))
+                                                (Etempvar _i tint)
+                                                (tptr tint)) tint)
+                                            (Ebinop Oadd
+                                              (Etempvar _t'10 tint)
+                                              (Etempvar _cost tint) tint)))
+                                        (Ssequence
+                                          (Sassign
+                                            (Ederef
+                                              (Ebinop Oadd
+                                                (Etempvar _prev (tptr tint))
+                                                (Etempvar _i tint)
+                                                (tptr tint)) tint)
+                                            (Etempvar _u tint))
                                           (Ssequence
-                                            (Sset _t'10
+                                            (Sset _t'8
                                               (Ederef
                                                 (Ebinop Oadd
-                                                  (Etempvar _dist (tptr tint))
+                                                  (Etempvar _keys (tptr tint))
                                                   (Etempvar _i tint)
                                                   (tptr tint)) tint))
-                                            (Scall None
-                                              (Evar _pq_edit_priority 
-                                              (Tfunction
-                                                (Tcons
-                                                  (tptr (Tstruct _structPQ noattr))
-                                                  (Tcons tint
-                                                    (Tcons tint Tnil))) tvoid
-                                                cc_default))
-                                              ((Etempvar _pq (tptr (Tstruct _structPQ noattr))) ::
-                                               (Etempvar _t'9 tint) ::
-                                               (Etempvar _t'10 tint) :: nil))))))
-                                    Sskip)))
-                              Sskip)))
-                        (Sset _i
-                          (Ebinop Oadd (Etempvar _i tint)
-                            (Econst_int (Int.repr 1) tint) tint))))))
+                                            (Ssequence
+                                              (Sset _t'9
+                                                (Ederef
+                                                  (Ebinop Oadd
+                                                    (Etempvar _dist (tptr tint))
+                                                    (Etempvar _i tint)
+                                                    (tptr tint)) tint))
+                                              (Scall None
+                                                (Evar _pq_edit_priority 
+                                                (Tfunction
+                                                  (Tcons
+                                                    (tptr (Tstruct _structPQ noattr))
+                                                    (Tcons tint
+                                                      (Tcons tint Tnil)))
+                                                  tvoid cc_default))
+                                                ((Etempvar _pq (tptr (Tstruct _structPQ noattr))) ::
+                                                 (Etempvar _t'8 tint) ::
+                                                 (Etempvar _t'9 tint) :: nil))))))
+                                      Sskip)))
+                                Sskip)))
+                          (Sset _i
+                            (Ebinop Oadd (Etempvar _i tint)
+                              (Econst_int (Int.repr 1) tint) tint)))))))
                 Sskip)
               (Ssequence
                 (Scall None
@@ -1193,17 +1195,18 @@ Definition global_definitions : list (ident * globdef fundef type) :=
    Gfun(External (EF_external "time"
                    (mksignature (AST.Tint :: nil) AST.Tint cc_default))
      (Tcons (tptr tint) Tnil) tint cc_default)) ::
+ (_pq_remove_min_nc,
+   Gfun(External (EF_external "pq_remove_min_nc"
+                   (mksignature (AST.Tint :: AST.Tint :: nil) AST.Tvoid
+                     cc_default))
+     (Tcons (tptr (Tstruct _structPQ noattr))
+       (Tcons (tptr (Tstruct _structItem noattr)) Tnil)) tvoid cc_default)) ::
  (_pq_insert_nc,
    Gfun(External (EF_external "pq_insert_nc"
                    (mksignature (AST.Tint :: AST.Tint :: AST.Tint :: nil)
                      AST.Tint cc_default))
      (Tcons (tptr (Tstruct _structPQ noattr)) (Tcons tint (Tcons tint Tnil)))
      tuint cc_default)) ::
- (_pq_remove_min,
-   Gfun(External (EF_external "pq_remove_min"
-                   (mksignature (AST.Tint :: nil) AST.Tint cc_default))
-     (Tcons (tptr (Tstruct _structPQ noattr)) Tnil)
-     (tptr (Tstruct _structItem noattr)) cc_default)) ::
  (_pq_edit_priority,
    Gfun(External (EF_external "pq_edit_priority"
                    (mksignature (AST.Tint :: AST.Tint :: AST.Tint :: nil)
@@ -1233,7 +1236,7 @@ Definition global_definitions : list (ident * globdef fundef type) :=
 Definition public_idents : list ident :=
 (_main :: _dijkstra :: _getCell :: _getPaths :: _printPath :: _print_graph ::
  _setup :: _pq_free :: _pq_make :: _pq_size :: _pq_edit_priority ::
- _pq_remove_min :: _pq_insert_nc :: _time :: _printf :: _srand :: _rand ::
+ _pq_insert_nc :: _pq_remove_min_nc :: _time :: _printf :: _srand :: _rand ::
  _free :: _malloc :: ___builtin_debug :: ___builtin_write32_reversed ::
  ___builtin_write16_reversed :: ___builtin_read32_reversed ::
  ___builtin_read16_reversed :: ___builtin_fnmsub :: ___builtin_fnmadd ::
